add code outline for communication analysis B

theory/Static_Communication_Analysis_A.thy
@@ -1,18 +1,10 @@
 theory Static_Communication_Analysis_A
   imports Main Syntax 
-    Dynamic_Semantics Static_Semantics
+    Dynamic_Semantics 
+    Static_Semantics
     Dynamic_Communication_Analysis
+    Static_Communication_Analysis
 begin
-
-datatype node_label = NLet var | NResult var
-
-fun nodeLabel :: "exp \<Rightarrow> node_label" where
-  "nodeLabel (LET x = b in e) = NLet x" |
-  "nodeLabel (RESULT y) = NResult y"
-
-type_synonym node_set = "node_label set"
-
-type_synonym node_map = "node_label \<Rightarrow> var set"
 
 datatype edge_label = ENext | ESpawn | ECall | EReturn
 
@@ -23,22 +15,6 @@ type_synonym flow_set = "flow_label set"
 type_synonym step_label = "(node_label \<times> edge_label)"
 
 type_synonym abstract_path = "step_label list"
-
-inductive may_be_static_send_node_label :: "abstract_value_env \<Rightarrow> exp \<Rightarrow> var \<Rightarrow> node_label \<Rightarrow> bool" where
-  Sync: "
-    {^Chan xC} \<subseteq> V xSC \<Longrightarrow>
-    {^Send_Evt xSC xM} \<subseteq> V xE \<Longrightarrow>
-    is_super_exp e (LET x = SYNC xE in e') \<Longrightarrow>
-    may_be_static_send_node_label V e xC (NLet x)
-  "
-
-inductive may_be_static_recv_node_label :: "abstract_value_env \<Rightarrow> exp \<Rightarrow> var \<Rightarrow> node_label \<Rightarrow> bool" where
-  Sync: "
-    {^Chan xC} \<subseteq> V xRC \<Longrightarrow>
-    {^Recv_Evt xRC} \<subseteq> V xE \<Longrightarrow>
-    is_super_exp e (LET x = SYNC xE in e') \<Longrightarrow>
-    may_be_static_recv_node_label V e xC (NLet x)
-  "
 
 
 inductive simple_flow_set :: "abstract_value_env \<Rightarrow> (node_label * edge_label * node_label) set \<Rightarrow> exp \<Rightarrow> bool"  where
@@ -240,41 +216,31 @@ inductive noncompetitive :: "abstract_path \<Rightarrow> abstract_path \<Rightar
     noncompetitive \<pi>\<^sub>1 \<pi>\<^sub>2
   "
 
-
-
-inductive every_two_abstract_paths  :: "(abstract_path \<Rightarrow> bool) \<Rightarrow> (abstract_path \<Rightarrow> abstract_path \<Rightarrow> bool) \<Rightarrow> bool" where
-  pred: "
-    (\<forall> path1 path2 . P path1 \<longrightarrow> P path2 \<longrightarrow> 
-      R path1 path2) \<Longrightarrow>
-    every_two_abstract_paths P R
-  "
-
-
 inductive static_one_shot :: "abstract_value_env \<Rightarrow> exp \<Rightarrow> var \<Rightarrow> bool" where
   Sync: "
-    every_two_abstract_paths (may_be_path V F (nodeLabel e) (may_be_static_send_node_label V e xC)) singular \<Longrightarrow>
+    every_two (may_be_path V F (nodeLabel e) (may_be_static_send_node_label V e xC)) singular \<Longrightarrow>
     simple_flow_set V F e \<Longrightarrow>
     static_one_shot V e xC 
   "
 
 inductive static_one_to_one :: "abstract_value_env \<Rightarrow> exp \<Rightarrow> var \<Rightarrow> bool" where
   Sync: "
-    every_two_abstract_paths (may_be_path V F (nodeLabel e) (may_be_static_send_node_label V e xC)) noncompetitive \<Longrightarrow>
-    every_two_abstract_paths (may_be_path V F (nodeLabel e) (may_be_static_recv_node_label V e xC)) noncompetitive \<Longrightarrow>
+    every_two (may_be_path V F (nodeLabel e) (may_be_static_send_node_label V e xC)) noncompetitive \<Longrightarrow>
+    every_two (may_be_path V F (nodeLabel e) (may_be_static_recv_node_label V e xC)) noncompetitive \<Longrightarrow>
     simple_flow_set V F e \<Longrightarrow>
     static_one_to_one V e xC 
   "
 
 inductive static_fan_out :: "abstract_value_env \<Rightarrow> exp \<Rightarrow> var \<Rightarrow> bool" where
   Sync: "
-    every_two_abstract_paths (may_be_path V F (nodeLabel e) (may_be_static_send_node_label V e xC)) noncompetitive \<Longrightarrow>
+    every_two (may_be_path V F (nodeLabel e) (may_be_static_send_node_label V e xC)) noncompetitive \<Longrightarrow>
     simple_flow_set V F e \<Longrightarrow>
     static_fan_out V e xC 
   "
 
 inductive static_fan_in :: "abstract_value_env \<Rightarrow> exp \<Rightarrow> var \<Rightarrow> bool" where
   Sync: "
-    every_two_abstract_paths (may_be_path V F (nodeLabel e) (may_be_static_recv_node_label V e xC)) noncompetitive \<Longrightarrow>
+    every_two (may_be_path V F (nodeLabel e) (may_be_static_recv_node_label V e xC)) noncompetitive \<Longrightarrow>
     simple_flow_set V F e \<Longrightarrow>
     static_fan_in V e xC 
   "
@@ -354,19 +320,6 @@ lemma paths_cong_preserved_under_reduction: "
   paths_congruent (\<pi> ;; l) (path @ [n]) \<Longrightarrow>
   paths_congruent \<pi> path"
 using paths_congruent.cases by fastforce
-
-
-lemma path_state_preserved_for_non_leaf: "
-(E, H) \<rightarrow> (E', H') \<Longrightarrow>
-E' (\<pi> ;; l) = Some \<sigma> \<Longrightarrow>
-\<not> leaf E \<pi> \<Longrightarrow>
-E (\<pi> ;; l) = Some \<sigma>
-"
-apply (erule concur_step.cases; auto; (erule seq_step.cases; auto)?)
-  apply presburger+
-  apply (metis append1_eq_conv fun_upd_other)
-  apply (metis butlast_snoc fun_upd_apply)
-done
 
 
 lemma equality_abstract_to_concrete': "
@@ -470,29 +423,6 @@ paths_congruent \<pi>2 path2 \<Longrightarrow>
 strict_prefix \<pi>1 \<pi>2
 "
 by (simp add: strict_prefix_abstract_to_concrete')
-
-lemma spawn_point: "
-  (E, H) \<rightarrow> (E', H') \<Longrightarrow>
-  leaf E \<pi> \<Longrightarrow>
-  E' (\<pi> ;; l1) = Some \<sigma>1 \<Longrightarrow>
-  E' (\<pi> ;; l2) = Some \<sigma>2 \<Longrightarrow>
-  l1 = l2 \<or> 
-  (\<exists> x . l1 = (LNext x) \<and> l2 = (LSpawn x)) \<or>
-  (\<exists> x . l1 = (LSpawn x) \<and> l2 = (LNext x))
-"
-apply (erule concur_step.cases; auto; (erule seq_step.cases; auto)?)
-  apply (metis leaf.cases option.distinct(1) strict_prefixI')
-  apply (metis leaf.cases option.distinct(1) strict_prefixI')
-  apply (metis leaf.cases option.distinct(1) strict_prefixI')
-  apply (metis leaf.cases option.distinct(1) strict_prefixI')
-  apply (metis leaf.cases option.distinct(1) strict_prefixI')
-  apply (metis leaf.cases option.distinct(1) strict_prefixI')
-  apply (metis leaf.cases option.distinct(1) strict_prefixI')
-  apply (metis (mono_tags, lifting) append1_eq_conv fun_upd_apply leaf.cases option.distinct(1) strict_prefixI')
-  apply (smt butlast_snoc exp.inject(1) fun_upd_apply last_snoc leaf.cases option.distinct(1) option.inject state.inject strict_prefixI')
-done
-
-
 
 
 lemma equality_contcrete_to_abstract': "
@@ -965,111 +895,6 @@ lemma isnt_path_sound: "
 by (metis lift_simple_flow_set_to_pool simple_flow_set_pool_implies_may_be_path simple_flow_set_pool_preserved_star)
 
 
-lemma isnt_send_evt_sound: "
-  \<lbrakk>
-    \<rho>\<^sub>y x\<^sub>e = Some (VClosure (Send_Evt x\<^sub>s\<^sub>c x\<^sub>m) \<rho>\<^sub>e);
-    ([[] \<mapsto> \<langle>e;Map.empty;[]\<rangle>], {}) \<rightarrow>* (\<E>', H');
-    \<E>' \<pi>\<^sub>y = Some (\<langle>LET x\<^sub>y = SYNC x\<^sub>e in e\<^sub>y;\<rho>\<^sub>y;\<kappa>\<^sub>y\<rangle>);
-    (V, C) \<Turnstile>\<^sub>e e
-  \<rbrakk> \<Longrightarrow>
-  {^Send_Evt x\<^sub>s\<^sub>c x\<^sub>m} \<subseteq> V x\<^sub>e
-"
-  apply (drule values_not_bound_sound; assumption?; auto)
-done
-
-lemma isnt_recv_evt_sound: "
-  \<lbrakk>
-    \<rho>\<^sub>y x\<^sub>e = Some (VClosure (Recv_Evt x\<^sub>r\<^sub>c) \<rho>\<^sub>e);
-    ([[] \<mapsto> \<langle>e;Map.empty;[]\<rangle>], {}) \<rightarrow>* (\<E>', H');
-    \<E>' \<pi>\<^sub>y = Some (\<langle>LET x\<^sub>y = SYNC x\<^sub>e in e\<^sub>y;\<rho>\<^sub>y;\<kappa>\<^sub>y\<rangle>);
-    (V, C) \<Turnstile>\<^sub>e e
-  \<rbrakk> \<Longrightarrow>
-  {^Recv_Evt x\<^sub>r\<^sub>c} \<subseteq> V x\<^sub>e
-"
-  apply (drule values_not_bound_sound; assumption?; auto)
-done
-
-lemma isnt_send_chan_sound: "
-  \<lbrakk>
-    \<rho>\<^sub>e x\<^sub>s\<^sub>c = Some (VChan (Ch \<pi> xC));
-    \<rho>\<^sub>y x\<^sub>e = Some (VClosure (Send_Evt x\<^sub>s\<^sub>c x\<^sub>m) \<rho>\<^sub>e);
-    \<E>' \<pi>\<^sub>y = Some (\<langle>LET x\<^sub>y = SYNC x\<^sub>e in e\<^sub>y;\<rho>\<^sub>y;\<kappa>\<^sub>y\<rangle>);
-    ([[] \<mapsto> \<langle>e;Map.empty;[]\<rangle>], {}) \<rightarrow>* (\<E>', H');
-    (V, C) \<Turnstile>\<^sub>e e
-  \<rbrakk> \<Longrightarrow> 
-  ^Chan xC \<in> V x\<^sub>s\<^sub>c
-"
- apply (frule may_be_static_eval_to_pool)
- apply (drule may_be_static_eval_preserved_under_concur_step_star[of _ _ _ ]; assumption?)
- apply (erule may_be_static_eval_pool.cases; auto)
- apply (drule spec[of _ \<pi>\<^sub>y], drule spec[of _ "\<langle>LET x\<^sub>y = SYNC x\<^sub>e in e\<^sub>y;\<rho>\<^sub>y;\<kappa>\<^sub>y\<rangle>"], simp)
- apply (erule may_be_static_eval_state.cases; auto)
- apply (erule may_be_static_eval_env.cases; auto)
- apply (drule spec[of _ x\<^sub>e], drule spec[of _ "(VClosure (Send_Evt x\<^sub>s\<^sub>c x\<^sub>m) \<rho>\<^sub>e)"]; simp)
- apply (erule conjE)
- apply (erule may_be_static_eval_value.cases; auto)
- apply (erule may_be_static_eval_env.cases; auto)
- apply (drule spec[of _ x\<^sub>s\<^sub>c], drule spec[of _ "(VChan (Ch \<pi> xC))"]; simp)
-done
-
-lemma isnt_recv_chan_sound: "
-  \<lbrakk>
-    \<rho>\<^sub>e x\<^sub>r\<^sub>c = Some (VChan (Ch \<pi> xC));
-    \<rho>\<^sub>y x\<^sub>e = Some (VClosure (Recv_Evt x\<^sub>r\<^sub>c) \<rho>\<^sub>e);
-    \<E>' \<pi>\<^sub>y = Some (\<langle>LET x\<^sub>y = SYNC x\<^sub>e in e\<^sub>y;\<rho>\<^sub>y;\<kappa>\<^sub>y\<rangle>);
-    ([[] \<mapsto> \<langle>e;Map.empty;[]\<rangle>], {}) \<rightarrow>* (\<E>', H');
-    (V, C) \<Turnstile>\<^sub>e e
-  \<rbrakk> \<Longrightarrow> 
-  ^Chan xC \<in> V x\<^sub>r\<^sub>c
-"
- apply (frule may_be_static_eval_to_pool)
- apply (drule may_be_static_eval_preserved_under_concur_step_star[of _ _ _ ]; assumption?)
- apply (erule may_be_static_eval_pool.cases; auto)
- apply (drule spec[of _ \<pi>\<^sub>y], drule spec[of _ "\<langle>LET x\<^sub>y = SYNC x\<^sub>e in e\<^sub>y;\<rho>\<^sub>y;\<kappa>\<^sub>y\<rangle>"], simp)
- apply (erule may_be_static_eval_state.cases; auto)
- apply (erule may_be_static_eval_env.cases; auto)
- apply (drule spec[of _ x\<^sub>e], drule spec[of _ "(VClosure (Recv_Evt x\<^sub>r\<^sub>c) \<rho>\<^sub>e)"]; simp)
- apply (erule conjE)
- apply (erule may_be_static_eval_value.cases; auto)
- apply (erule may_be_static_eval_env.cases; auto)
- apply (drule spec[of _ x\<^sub>r\<^sub>c], drule spec[of _ "(VChan (Ch \<pi> xC))"]; simp)
-done
-
-lemma isnt_send_site_sound: "
-  \<E>' \<pi>Sync = Some (\<langle>LET x\<^sub>y = SYNC x\<^sub>e in e\<^sub>n;\<rho>;\<kappa>\<rangle>) \<Longrightarrow>
-  \<rho> x\<^sub>e = Some (VClosure (Send_Evt x\<^sub>s\<^sub>c x\<^sub>m) \<rho>\<^sub>e) \<Longrightarrow>
-  \<rho>\<^sub>e x\<^sub>s\<^sub>c = Some (VChan (Ch \<pi>C xC)) \<Longrightarrow>
-  ([[] \<mapsto> \<langle>e;Map.empty;[]\<rangle>], {}) \<rightarrow>* (\<E>', H') \<Longrightarrow> 
-  (V, C) \<Turnstile>\<^sub>e e \<Longrightarrow>
-  may_be_static_send_node_label V e xC (NLet x\<^sub>y)
-"
- apply (unfold may_be_static_send_node_label.simps; auto)
- apply (rule exI[of _ x\<^sub>s\<^sub>c]; auto)
- apply (auto simp: isnt_send_chan_sound)
- apply (rule exI[of _ x\<^sub>m]; auto?)
- apply (rule exI[of _ x\<^sub>e]; auto?)
- apply (blast dest: isnt_send_evt_sound)
- apply (rule exI; auto?)
- apply (erule isnt_exp_sound; auto)
-done
-
-lemma isnt_recv_site_sound: "
-  \<E>' \<pi>Sync = Some (\<langle>LET x\<^sub>y = SYNC x\<^sub>e in e\<^sub>n;\<rho>;\<kappa>\<rangle>) \<Longrightarrow>
-  \<rho> x\<^sub>e = Some (VClosure (Recv_Evt x\<^sub>r\<^sub>c) \<rho>\<^sub>e) \<Longrightarrow>
-  \<rho>\<^sub>e x\<^sub>r\<^sub>c = Some (VChan (Ch \<pi>C xC)) \<Longrightarrow>
-  ([[] \<mapsto> \<langle>e;Map.empty;[]\<rangle>], {}) \<rightarrow>* (\<E>', H') \<Longrightarrow> 
-  (V, C) \<Turnstile>\<^sub>e e \<Longrightarrow>
-  may_be_static_recv_node_label V e xC (NLet x\<^sub>y)
-"
- apply (unfold may_be_static_recv_node_label.simps; auto)
- apply (rule exI[of _ x\<^sub>r\<^sub>c]; auto)
- apply (auto simp: isnt_recv_chan_sound)
- apply (rule exI[of _ x\<^sub>e]; auto?)
- apply (blast dest: isnt_recv_evt_sound)
- apply (rule exI; auto?)
- apply (erule isnt_exp_sound; auto)
-done
-
 
 lemma isnt_send_path_sound: "
   is_send_path \<E>' (Ch \<pi>C xC) \<pi>Sync \<Longrightarrow>
@@ -1104,13 +929,13 @@ done
 
 
 theorem one_shot_sound': "
-  every_two_abstract_paths (may_be_path V F (nodeLabel e) (may_be_static_send_node_label V e xC)) singular \<Longrightarrow>
+  every_two (may_be_path V F (nodeLabel e) (may_be_static_send_node_label V e xC)) singular \<Longrightarrow>
   simple_flow_set V F e \<Longrightarrow>
   (V, C) \<Turnstile>\<^sub>e e \<Longrightarrow>
   ([[] \<mapsto> \<langle>e;Map.empty;[]\<rangle>], {}) \<rightarrow>* (\<E>', H') \<Longrightarrow>
   every_two_dynamic_paths (is_send_path \<E>' (Ch \<pi> xC)) op =
 "
- apply (simp add: every_two_dynamic_paths.simps every_two_abstract_paths.simps singular.simps; auto)
+ apply (simp add: every_two_dynamic_paths.simps every_two.simps singular.simps; auto)
 
  apply (frule_tac \<pi>Sync = \<pi>\<^sub>1 in isnt_send_path_sound; auto)
  apply (drule_tac x = pathSync in spec)
@@ -1135,13 +960,13 @@ done
 
 
 theorem noncompetitive_send_to_ordered_send: "
-  every_two_abstract_paths (may_be_path V F (nodeLabel e) (may_be_static_send_node_label V e xC)) noncompetitive \<Longrightarrow>
+  every_two (may_be_path V F (nodeLabel e) (may_be_static_send_node_label V e xC)) noncompetitive \<Longrightarrow>
   simple_flow_set V F e \<Longrightarrow>
   (V, C) \<Turnstile>\<^sub>e e \<Longrightarrow>
   ([[] \<mapsto> \<langle>e;Map.empty;[]\<rangle>], {}) \<rightarrow>* (\<E>', H') \<Longrightarrow>
   every_two_dynamic_paths (is_send_path \<E>' (Ch \<pi> xC)) ordered
 "
-apply (simp add: every_two_abstract_paths.simps noncompetitive.simps; auto?)
+apply (simp add: every_two.simps noncompetitive.simps; auto?)
 apply (simp add: every_two_dynamic_paths.simps; auto)
   using isnt_send_path_sound abstract_paths_of_same_run_inclusive 
   apply (meson is_send_path_implies_nonempty_pool prefix_abstract_to_concrete)
@@ -1161,13 +986,13 @@ theorem fan_out_sound: "
 done
 
 lemma noncompetitive_recv_to_ordered_recv: "
-   every_two_abstract_paths (may_be_path V F (nodeLabel e) (may_be_static_recv_node_label V e xC)) noncompetitive \<Longrightarrow>
+   every_two (may_be_path V F (nodeLabel e) (may_be_static_recv_node_label V e xC)) noncompetitive \<Longrightarrow>
    simple_flow_set V F e \<Longrightarrow>
    (V, C) \<Turnstile>\<^sub>e e \<Longrightarrow>
    ([[] \<mapsto> \<langle>e;Map.empty;[]\<rangle>], {}) \<rightarrow>* (\<E>', H') \<Longrightarrow>
    every_two_dynamic_paths (is_recv_path \<E>' (Ch \<pi> xC)) ordered
 "
-apply (simp add: every_two_abstract_paths.simps noncompetitive.simps; auto?)
+apply (simp add: every_two.simps noncompetitive.simps; auto?)
 apply (simp add: every_two_dynamic_paths.simps; auto)
   using isnt_recv_path_sound abstract_paths_of_same_run_inclusive 
 apply (meson is_recv_path_implies_nonempty_pool prefix_abstract_to_concrete)
