theory/Static_Communication_Analysis_B.thy
@@ -1,13 +1,19 @@
-theory Static_Communication_Analysis
+theory Static_Communication_Analysis_B
   imports Main Syntax 
-    Dynamic_Semantics Static_Semantics Sound_Semantics
-    Static_Framework Sound_Framework
+    Dynamic_Semantics Static_Semantics
     Dynamic_Communication_Analysis 
+    Static_Communication_Analysis 
 begin
 
-(*
+datatype edge_label = ENext | ESpawn | ECall | EReturn var
 
+type_synonym flow_label = "(node_label \<times> edge_label \<times> node_label)"
 
+type_synonym flow_set = "flow_label set"
+
+type_synonym step_label = "(node_label \<times> edge_label)"
+
+type_synonym abstract_path = "step_label list"
 
 
 inductive static_flow_set :: "abstract_value_env \<Rightarrow> flow_set \<Rightarrow> (var \<Rightarrow> node_label \<Rightarrow> bool) \<Rightarrow> exp \<Rightarrow> bool"  where
@@ -112,8 +118,8 @@ inductive static_flow_set :: "abstract_value_env \<Rightarrow> flow_set \<Righta
   Let_Case: "
     \<lbrakk>
       {
-        (NLet x, ECall x, nodeLabel e\<^sub>l),
-        (NLet x, ECall x, nodeLabel e\<^sub>r),
+        (NLet x, ECall, nodeLabel e\<^sub>l),
+        (NLet x, ECall, nodeLabel e\<^sub>r),
         (NResult (\<lfloor>e\<^sub>l\<rfloor>), EReturn x, nodeLabel e),
         (NResult (\<lfloor>e\<^sub>r\<rfloor>), EReturn x, nodeLabel e)
       } \<subseteq> F;
@@ -127,7 +133,7 @@ inductive static_flow_set :: "abstract_value_env \<Rightarrow> flow_set \<Righta
     \<lbrakk>
       (\<forall> f' x\<^sub>p e\<^sub>b . ^Abs f' x\<^sub>p e\<^sub>b \<in> V f \<longrightarrow>
         {
-          (NLet x, ECall x, nodeLabel e\<^sub>b),
+          (NLet x, ECall, nodeLabel e\<^sub>b),
           (NResult (\<lfloor>e\<^sub>b\<rfloor>), EReturn x, nodeLabel e)
         } \<subseteq> F);
       static_flow_set V F may_be_recv_site e
@@ -330,41 +336,41 @@ inductive static_chan_liveness :: "abstract_value_env \<Rightarrow> node_map \<R
 
 
 
-inductive may_be_static_path :: "flow_set \<Rightarrow> node_label \<Rightarrow> static_path \<Rightarrow> bool" where
+inductive may_be_abstract_path :: "flow_set \<Rightarrow> node_label \<Rightarrow> abstract_path \<Rightarrow> bool" where
   Empty: "
-    may_be_static_path F end []
+    may_be_abstract_path F end []
   " |
   Edge: "
     (start, edge, end) \<in> F \<Longrightarrow>
-    may_be_static_path F end [(start, edge)]
+    may_be_abstract_path F end [(start, edge)]
   " |
   Step: "
-    may_be_static_path F end ((middle, edge') # post) \<Longrightarrow>
+    may_be_abstract_path F end ((middle, edge') # post) \<Longrightarrow>
     (start, edge, middle) \<in> F \<Longrightarrow>
     path = [(start, edge), (middle, edge')] @ post \<Longrightarrow>
-    may_be_static_path F end path
+    may_be_abstract_path F end path
   "
 
-inductive static_balanced :: "static_path \<Rightarrow> bool" where
+inductive abstract_balanced :: "abstract_path \<Rightarrow> bool" where
   Empty: "
-    static_balanced []
+    abstract_balanced []
   " |
   Next: "
-    static_balanced [(NLet x, ENext)]
+    abstract_balanced [(NLet x, ENext)]
   " |
   CallReturn: "
-    static_balanced path \<Longrightarrow>
-    static_balanced ((NLet x, ECall x) # (path @ [(NResult y, EReturn x)]))
+    abstract_balanced path \<Longrightarrow>
+    abstract_balanced ((NLet x, ECall) # (path @ [(NResult y, EReturn x)]))
   " |
   Append: "
     path \<noteq> [] \<Longrightarrow>
-    static_balanced path \<Longrightarrow>
+    abstract_balanced path \<Longrightarrow>
     path' \<noteq> [] \<Longrightarrow>
-    static_balanced path' \<Longrightarrow>
-    static_balanced (path @ path')
+    abstract_balanced path' \<Longrightarrow>
+    abstract_balanced (path @ path')
   "
 
-inductive static_unbalanced :: "static_path \<Rightarrow> bool" where
+inductive static_unbalanced :: "abstract_path \<Rightarrow> bool" where
   Result: "
     static_unbalanced ((NResult y, EReturn x) # post)
   " |
@@ -388,14 +394,14 @@ inductive may_be_static_live_flow :: "flow_set \<Rightarrow> node_map \<Rightarr
     may_be_static_live_flow F Ln Lx (l, ESpawn, l')
   " |
   Call_Live_Outer: "
-    (l, ECall x, l') \<in> F \<Longrightarrow>
+    (l, ECall, l') \<in> F \<Longrightarrow>
     \<not> Set.is_empty (Lx l) \<Longrightarrow>
-    may_be_static_live_flow F Ln Lx (l, ECall x, l')
+    may_be_static_live_flow F Ln Lx (l, ECall, l')
   " |
   Call_Live_Inner: "
-    (l, ECall x, l') \<in> F \<Longrightarrow>
+    (l, ECall, l') \<in> F \<Longrightarrow>
     \<not> Set.is_empty (Ln l') \<Longrightarrow>
-    may_be_static_live_flow F Ln Lx (l, ECall x, l')
+    may_be_static_live_flow F Ln Lx (l, ECall, l')
   " |
   Return: "
     (l, EReturn x, l') \<in> F \<Longrightarrow>
@@ -408,7 +414,7 @@ inductive may_be_static_live_flow :: "flow_set \<Rightarrow> node_map \<Rightarr
     may_be_static_live_flow F Ln Lx ((NLet xSend), ESend xE, (NLet xRecv))
   "
 
-inductive may_be_static_live_path :: "abstract_value_env \<Rightarrow> flow_set \<Rightarrow> node_map \<Rightarrow> node_map \<Rightarrow> node_label \<Rightarrow> (node_label \<Rightarrow> bool) \<Rightarrow> static_path \<Rightarrow> bool" where
+inductive may_be_static_live_path :: "abstract_value_env \<Rightarrow> flow_set \<Rightarrow> node_map \<Rightarrow> node_map \<Rightarrow> node_label \<Rightarrow> (node_label \<Rightarrow> bool) \<Rightarrow> abstract_path \<Rightarrow> bool" where
   Empty: "
     isEnd start \<Longrightarrow>
     may_be_static_live_path V F Ln Lx start isEnd []
@@ -426,104 +432,30 @@ inductive may_be_static_live_path :: "abstract_value_env \<Rightarrow> flow_set 
 
   Pre_Return: "
     may_be_static_live_path V F Ln Lx (NResult y) isEnd ((NResult y, EReturn x) # post) \<Longrightarrow>
-    may_be_static_path  F (NResult y) pre \<Longrightarrow>
-    \<not> static_balanced (pre @ [(NResult y, EReturn x)]) \<Longrightarrow>
+    may_be_abstract_path  F (NResult y) pre \<Longrightarrow>
+    \<not> abstract_balanced (pre @ [(NResult y, EReturn x)]) \<Longrightarrow>
     \<not> Set.is_empty (Lx (NLet x)) \<Longrightarrow>
     path = pre @ (NResult y, EReturn x) # post \<Longrightarrow>
     may_be_static_live_path V F Ln Lx start isEnd path
   "
 
-(*
-
-inductive may_be_inclusive :: "static_path \<Rightarrow> static_path \<Rightarrow> bool" (infix "\<asymp>" 55) where
-  Prefix1: "
-    prefix \<pi>\<^sub>1 \<pi>\<^sub>2 \<Longrightarrow>
-    \<pi>\<^sub>1 \<asymp> \<pi>\<^sub>2
-  " |
-  Prefix2: "
-    prefix \<pi>\<^sub>2 \<pi>\<^sub>1 \<Longrightarrow>
-    \<pi>\<^sub>1 \<asymp> \<pi>\<^sub>2
-  " |
-  Spawn1: "
-    \<pi> @ (NLet x, ESpawn) # \<pi>\<^sub>1 \<asymp> \<pi> @ (NLet x, ENext) # \<pi>\<^sub>2
-  " |
-  Spawn2: "
-    \<pi> @ (NLet x, ENext) # \<pi>\<^sub>1 \<asymp> \<pi> @ (NLet x, ESpawn) # \<pi>\<^sub>2
-  " |
-  Send1: "
-    \<pi> @ (NLet x, ESend xE) # \<pi>\<^sub>1 \<asymp> \<pi> @ (NLet x, ENext) # \<pi>\<^sub>2
-  " |
-  Send2: "
-    \<pi> @ (NLet x, ENext) # \<pi>\<^sub>1 \<asymp> \<pi> @ (NLet x, ESend xE) # \<pi>\<^sub>2
-  " |
-  Kite: "
-    p1 @ [(NLet x1, ESend xE1)] \<noteq> (p2 @ [(NLet x2, ESend xE2)]) \<Longrightarrow>
-    ((NLet x, ENext) # p1 @ [(NLet x1, ESend xE1)] @ p1') \<asymp> 
-      ((NLet x, ENext) # p2 @ [(NLet x2, ESend xE2)] @ p2')
-  "
-
-lemma may_be_inclusive_commut: "
-  path\<^sub>1 \<asymp> path\<^sub>2 \<Longrightarrow> path\<^sub>2 \<asymp> path\<^sub>1
-"
- apply (erule may_be_inclusive.cases; auto)
-  apply (simp add: Prefix2)
-  apply (simp add: Prefix1)
-  apply (simp add: Spawn2)
-  apply (simp add: Spawn1)
-  apply (simp add: Send2)
-  apply (simp add: Send1)
-  using Kite apply auto[1]
-  using Kite apply auto[1]
-  using Kite apply auto[1]
-done
-
-
-lemma may_be_inclusive_preserved_under_unordered_extension: "
-  \<not> prefix path\<^sub>1 path\<^sub>2 \<Longrightarrow> \<not> prefix path\<^sub>2 path\<^sub>1 \<Longrightarrow> path\<^sub>1 \<asymp> path\<^sub>2 \<Longrightarrow> path\<^sub>1 @ [l] \<asymp> path\<^sub>2
-"
- apply (erule may_be_inclusive.cases; auto)
-  apply (simp add: Spawn1)
-  apply (simp add: Spawn2)
-  apply (simp add: Send1)
-  apply (simp add: Send2)
-  using Kite apply auto[1]
-  using Kite apply auto[1]
-  using Kite apply auto
-done
-
-lemma may_be_inclusive_preserved_under_unordered_double_extension: "
-  path\<^sub>1 \<asymp> path\<^sub>2 \<Longrightarrow> \<not> prefix path\<^sub>1 path\<^sub>2 \<Longrightarrow> \<not> prefix path\<^sub>2 path\<^sub>1 \<Longrightarrow> path\<^sub>1 @ [l1] \<asymp> path\<^sub>2 @ [l2]
-"
-by (metis may_be_inclusive_commut may_be_inclusive_preserved_under_unordered_extension prefix_append prefix_def)
-
-*)
-
-inductive singular :: "static_path \<Rightarrow> static_path \<Rightarrow> bool" where
+inductive singular :: "abstract_path \<Rightarrow> abstract_path \<Rightarrow> bool" where
   equal: "
     \<pi>\<^sub>1 = \<pi>\<^sub>2 \<Longrightarrow> 
     singular \<pi>\<^sub>1 \<pi>\<^sub>2
   "
-(*|
-  exclusive: "
-    \<not> (\<pi>\<^sub>1 \<asymp> \<pi>\<^sub>2) \<Longrightarrow> 
-    singular \<pi>\<^sub>1 \<pi>\<^sub>2
-  "*)
 
-inductive noncompetitive :: "static_path \<Rightarrow> static_path \<Rightarrow> bool" where
+inductive noncompetitive :: "abstract_path \<Rightarrow> abstract_path \<Rightarrow> bool" where
   ordered: "
     ordered \<pi>\<^sub>1 \<pi>\<^sub>2 \<Longrightarrow> 
     noncompetitive \<pi>\<^sub>1 \<pi>\<^sub>2
-  " (*|
-  exclusive: "
-    \<not> (\<pi>\<^sub>1 \<asymp> \<pi>\<^sub>2) \<Longrightarrow> 
-    noncompetitive \<pi>\<^sub>1 \<pi>\<^sub>2
-  "*)
+  "
 
 
 
 inductive static_one_shot :: "abstract_value_env \<Rightarrow> exp \<Rightarrow> var \<Rightarrow> bool" where
   Sync: "
-    every_two_static_paths (may_be_static_live_path V F Ln Lx (NLet xC) (may_be_static_send_node_label V e xC)) singular \<Longrightarrow>
+    every_two (may_be_static_live_path V F Ln Lx (NLet xC) (may_be_static_send_node_label V e xC)) singular \<Longrightarrow>
     static_chan_liveness V Ln Lx xC e \<Longrightarrow>
     static_flow_set V F (may_be_static_recv_node_label V e) e \<Longrightarrow>
     static_one_shot V e xC 
@@ -531,8 +463,8 @@ inductive static_one_shot :: "abstract_value_env \<Rightarrow> exp \<Rightarrow>
 
 inductive static_one_to_one :: "abstract_value_env \<Rightarrow> exp \<Rightarrow> var \<Rightarrow> bool" where
   Sync: "
-    every_two_static_paths (may_be_static_live_path V F Ln Lx (NLet xC) (may_be_static_send_node_label V e xC)) noncompetitive \<Longrightarrow>
-    every_two_static_paths (may_be_static_live_path V F Ln Lx (NLet xC) (may_be_static_recv_node_label V e xC)) noncompetitive \<Longrightarrow>
+    every_two (may_be_static_live_path V F Ln Lx (NLet xC) (may_be_static_send_node_label V e xC)) noncompetitive \<Longrightarrow>
+    every_two (may_be_static_live_path V F Ln Lx (NLet xC) (may_be_static_recv_node_label V e xC)) noncompetitive \<Longrightarrow>
     static_chan_liveness V Ln Lx xC e \<Longrightarrow>
     static_flow_set V F (may_be_static_recv_node_label V e) e \<Longrightarrow>
     static_one_to_one V e xC 
@@ -540,7 +472,7 @@ inductive static_one_to_one :: "abstract_value_env \<Rightarrow> exp \<Rightarro
 
 inductive static_fan_out :: "abstract_value_env \<Rightarrow> exp \<Rightarrow> var \<Rightarrow> bool" where
   Sync: "
-    every_two_static_paths (may_be_static_live_path V F Ln Lx (NLet xC) (may_be_static_send_node_label V e xC)) noncompetitive \<Longrightarrow>
+    every_two (may_be_static_live_path V F Ln Lx (NLet xC) (may_be_static_send_node_label V e xC)) noncompetitive \<Longrightarrow>
     static_chan_liveness V Ln Lx xC e \<Longrightarrow>
     static_flow_set V F (may_be_static_recv_node_label V e) e \<Longrightarrow>
     static_fan_out V e xC 
@@ -548,188 +480,11 @@ inductive static_fan_out :: "abstract_value_env \<Rightarrow> exp \<Rightarrow> 
 
 inductive static_fan_in :: "abstract_value_env \<Rightarrow> exp \<Rightarrow> var \<Rightarrow> bool" where
   Sync: "
-    every_two_static_paths (may_be_static_live_path V F Ln Lx (NLet xC) (may_be_static_recv_node_label V e xC)) noncompetitive \<Longrightarrow>
+    every_two (may_be_static_live_path V F Ln Lx (NLet xC) (may_be_static_recv_node_label V e xC)) noncompetitive \<Longrightarrow>
     static_chan_liveness V Ln Lx xC e \<Longrightarrow>
     static_flow_set V F (may_be_static_recv_node_label V e) e \<Longrightarrow>
     static_fan_in V e xC 
   "
-
-
-
-
-
-
-
-
-
-
-
-
-
-
-
-
-
-
-(*
-
-
-lemma inclusive_preserved: "
-  \<E> \<rightarrow> \<E>' \<Longrightarrow>
-  \<forall>\<pi>1. (\<exists>\<sigma>\<^sub>1. \<E> \<pi>1 = Some \<sigma>\<^sub>1) \<longrightarrow> (\<forall>\<pi>2. (\<exists>\<sigma>\<^sub>2. \<E> \<pi>2 = Some \<sigma>\<^sub>2) \<longrightarrow> \<pi>1 \<asymp> \<pi>2) \<Longrightarrow>
-  \<E>' \<pi>1 = Some \<sigma>\<^sub>1 \<Longrightarrow> \<E>' \<pi>2 = Some \<sigma>\<^sub>2 \<Longrightarrow> 
-  \<pi>1 \<asymp> \<pi>2
-"
- apply (erule concur_step.cases; auto; (erule seq_step.cases; auto)?)
-
-   apply (case_tac "\<pi>1 = \<pi> ;; (LReturn x\<^sub>\<kappa>')"; auto; (case_tac "\<pi>2 = \<pi> ;; (LReturn x\<^sub>\<kappa>')"; auto))
-   apply (simp add: Ordered)
-   apply (metis Ordered inclusive_preserved_under_unordered_extension leaf.simps option.distinct(1) prefix_order.dual_order.order_iff_strict prefix_snoc)
-   apply (metis Ordered inclusive_commut inclusive_preserved_under_unordered_extension leaf.simps prefix_append prefix_order.dual_order.order_iff_strict)
-
-   apply (case_tac "\<pi>1 = \<pi> ;; (LNext xa)"; auto; (case_tac "\<pi>2 = \<pi> ;; (LNext xa)"; auto))
-   apply (simp add: Ordered)
-   apply (metis Ordered inclusive_preserved_under_unordered_extension leaf.simps option.distinct(1) prefix_order.dual_order.order_iff_strict prefix_snoc)
-   apply (metis Ordered inclusive_commut inclusive_preserved_under_unordered_extension leaf.simps prefix_append prefix_order.dual_order.order_iff_strict)
-
-
-   apply (case_tac "\<pi>1 = \<pi> ;; (LNext xa)"; auto; (case_tac "\<pi>2 = \<pi> ;; (LNext xa)"; auto))
-   apply (simp add: Ordered)
-   apply (metis Ordered inclusive_preserved_under_unordered_extension leaf.simps option.distinct(1) prefix_order.dual_order.order_iff_strict prefix_snoc)
-   apply (metis Ordered inclusive_commut inclusive_preserved_under_unordered_extension leaf.simps prefix_append prefix_order.dual_order.order_iff_strict)
-
-   apply (case_tac "\<pi>1 = \<pi> ;; (LNext xa)"; auto; (case_tac "\<pi>2 = \<pi> ;; (LNext xa)"; auto))
-   apply (simp add: Ordered)
-   apply (metis Ordered inclusive_preserved_under_unordered_extension leaf.simps option.distinct(1) prefix_order.dual_order.order_iff_strict prefix_snoc)
-   apply (metis Ordered inclusive_commut inclusive_preserved_under_unordered_extension leaf.simps prefix_append prefix_order.dual_order.order_iff_strict)
-
-   apply (case_tac "\<pi>1 = \<pi> ;; (LNext xa)"; auto; (case_tac "\<pi>2 = \<pi> ;; (LNext xa)"; auto))
-   apply (simp add: Ordered)
-   apply (metis Ordered inclusive_preserved_under_unordered_extension leaf.simps option.distinct(1) prefix_order.dual_order.order_iff_strict prefix_snoc)
-   apply (metis Ordered inclusive_commut inclusive_preserved_under_unordered_extension leaf.simps prefix_append prefix_order.dual_order.order_iff_strict)
-
-
-   apply (case_tac "\<pi>1 = \<pi> ;; (LCall xa)"; auto; (case_tac "\<pi>2 = \<pi> ;; (LCall xa)"; auto))
-   apply (simp add: Ordered)
-   apply (metis Ordered inclusive_preserved_under_unordered_extension leaf.simps option.distinct(1) prefix_order.dual_order.order_iff_strict prefix_snoc)
-   apply (metis Ordered inclusive_commut inclusive_preserved_under_unordered_extension leaf.simps prefix_append prefix_order.dual_order.order_iff_strict)
-
-   apply (case_tac "\<pi>1 = \<pi> ;; (LCall xa)"; auto; (case_tac "\<pi>2 = \<pi> ;; (LCall xa)"; auto))
-   apply (simp add: Ordered)
-   apply (metis Ordered inclusive_preserved_under_unordered_extension leaf.simps option.distinct(1) prefix_order.dual_order.order_iff_strict prefix_snoc)
-   apply (metis Ordered inclusive_commut inclusive_preserved_under_unordered_extension leaf.simps prefix_append prefix_order.dual_order.order_iff_strict)
-   
-   apply (case_tac "\<pi>1 = \<pi> ;; (LCall xa)"; auto; (case_tac "\<pi>2 = \<pi> ;; (LCall xa)"; auto))
-   apply (simp add: Ordered)
-   apply (metis Ordered inclusive_preserved_under_unordered_extension leaf.simps option.distinct(1) prefix_order.dual_order.order_iff_strict prefix_snoc)
-   apply (metis Ordered inclusive_commut inclusive_preserved_under_unordered_extension leaf.simps prefix_append prefix_order.dual_order.order_iff_strict)
-
-   apply (case_tac "\<pi>1 = \<pi> ;; (LNext x)"; auto; (case_tac "\<pi>2 = \<pi> ;; (LNext x)"; auto))
-   apply (simp add: Ordered)
-   apply (metis Ordered inclusive_preserved_under_unordered_extension leaf.simps option.distinct(1) prefix_order.dual_order.order_iff_strict prefix_snoc)
-   apply (metis Ordered inclusive_commut inclusive_preserved_under_unordered_extension leaf.simps prefix_append prefix_order.dual_order.order_iff_strict)
-
-   apply (case_tac "\<pi>1 = \<pi> ;; (LSpawn x)"; auto; (case_tac "\<pi>2 = \<pi> ;; (LSpawn x)"; auto))
-   apply (simp add: Ordered)
-   apply (case_tac "\<pi>2 = \<pi> ;; (LNext x)"; auto)
-  apply (simp add: Spawn_Left)
-  apply (metis Ordered inclusive_preserved_under_unordered_extension leaf.simps option.distinct(1) prefix_order.dual_order.order_iff_strict prefix_snoc)
-  apply (case_tac "\<pi>1 = \<pi> ;; (LNext x)"; auto)
-  apply (simp add: Spawn_Right)
-  apply (metis Ordered inclusive_commut inclusive_preserved_under_unordered_extension leaf.simps prefix_append prefix_order.dual_order.order_iff_strict) 
-   apply (case_tac "\<pi>1 = \<pi> ;; (LNext x)"; auto; (case_tac "\<pi>2 = \<pi> ;; (LNext x)"; auto))
-   apply (simp add: Ordered)
-   apply (metis Ordered inclusive_preserved_under_unordered_extension leaf.simps option.distinct(1) prefix_order.dual_order.order_iff_strict prefix_snoc)
-   apply (metis Ordered inclusive_commut inclusive_preserved_under_unordered_extension leaf.simps prefix_append prefix_order.dual_order.order_iff_strict)
-
-
-   apply (case_tac "\<pi>1 = \<pi>\<^sub>r ;; (LNext x\<^sub>r)"; auto)
-   apply (case_tac "\<pi>2 = \<pi>\<^sub>r ;; (LNext x\<^sub>r)"; auto)
-   apply (simp add: Ordered)
-   apply (case_tac "\<pi>2 = \<pi>\<^sub>s ;; (LNext x\<^sub>s)"; auto)
-   apply (metis inclusive.simps inclusive_preserved_under_unordered_extension leaf.simps prefix_order.dual_order.not_eq_order_implies_strict prefix_snoc)
-   apply (drule_tac x = \<pi>\<^sub>r in spec; auto)
-   apply (drule_tac x = \<pi>\<^sub>s in spec; auto)
-   apply (smt Ordered exp.inject(1) inclusive_commut inclusive_preserved_under_unordered_extension leaf.simps option.inject prefix_order.dual_order.not_eq_order_implies_strict prefix_snoc state.inject)
-   apply (drule_tac x = \<pi>\<^sub>r in spec; auto)
-   apply (drule_tac x = \<pi>2 in spec; auto)
-   apply (metis Ordered inclusive_preserved_under_unordered_extension leaf.simps option.simps(3) prefix_order.le_less prefix_snoc)
-   apply (case_tac "\<pi>1 = \<pi>\<^sub>s ;; (LNext x\<^sub>s)"; auto)
-   apply (case_tac "\<pi>2 = \<pi>\<^sub>r ;; (LNext x\<^sub>r)"; auto)
-   apply (metis inclusive.simps inclusive_preserved_under_unordered_extension leaf.simps prefix_order.dual_order.not_eq_order_implies_strict prefix_snoc)
-   apply (case_tac "\<pi>2 = \<pi>\<^sub>s ;; (LNext x\<^sub>s)"; auto)
-   apply (simp add: Ordered)
-   apply (drule_tac x = \<pi>\<^sub>s in spec; auto)
-   apply (drule_tac x = \<pi>2 in spec; auto)
-   apply (metis Ordered inclusive_preserved_under_unordered_extension leaf.simps option.distinct(1) prefix_order.dual_order.not_eq_order_implies_strict prefix_snoc)
-   apply (case_tac "\<pi>2 = \<pi>\<^sub>r ;; (LNext x\<^sub>r)"; auto)
-   apply (drule_tac x = \<pi>\<^sub>r in spec; auto)
-   apply (drule_tac x = \<pi>\<^sub>s in spec; auto)
-   apply (smt Ordered exp.inject(1) inclusive_commut inclusive_preserved_under_unordered_extension leaf.simps option.inject prefix_order.dual_order.not_eq_order_implies_strict prefix_snoc state.inject)
-   apply (case_tac "\<pi>2 = \<pi>\<^sub>s ;; (LNext x\<^sub>s)"; auto)
-   apply (simp add: Ordered)
-   apply (drule_tac x = \<pi>\<^sub>s in spec; auto)
-   apply (drule_tac x = \<pi>2 in spec; auto)
-   apply (metis Ordered inclusive_preserved_under_unordered_extension leaf.simps option.simps(3) prefix_order.le_less prefix_snoc)
-   apply (case_tac "\<pi>2 = \<pi>\<^sub>r ;; (LNext x\<^sub>r)"; auto)
-   apply (drule_tac x = \<pi>\<^sub>r in spec; auto)
-   apply (drule_tac x = \<pi>1 in spec; auto)
-   apply (metis Ordered inclusive_commut inclusive_preserved_under_unordered_extension leaf.simps option.distinct(1) prefix_order.dual_order.not_eq_order_implies_strict prefix_snoc)
-   apply (case_tac "\<pi>2 = \<pi>\<^sub>s ;; (LNext x\<^sub>s)"; auto)
-   apply (drule_tac x = \<pi>\<^sub>s in spec; auto)
-   apply (drule_tac x = \<pi>1 in spec; auto)
-   apply (metis Ordered inclusive_commut inclusive_preserved_under_unordered_extension leaf.simps option.distinct(1) prefix_order.dual_order.not_eq_order_implies_strict prefix_snoc)
-   apply (drule_tac x = \<pi>\<^sub>s in spec; auto)
-   apply (drule_tac x = \<pi>1 in spec; auto)
-   apply (metis Ordered inclusive_commut inclusive_preserved_under_unordered_extension leaf.simps option.distinct(1) prefix_order.dual_order.not_eq_order_implies_strict prefix_snoc)
- 
-done
-
-
-lemma runtime_paths_are_inclusive': "
-  \<E>\<^sub>0 \<rightarrow>* \<E> \<Longrightarrow>
-  (\<forall> \<pi>1 \<pi>2 \<sigma>\<^sub>1 \<sigma>\<^sub>2.
-    \<E>\<^sub>0 = [[] \<mapsto> \<langle>e\<^sub>0;Map.empty;[]\<rangle>] \<longrightarrow>
-    \<E> \<pi>1 = Some \<sigma>\<^sub>1 \<longrightarrow>
-    \<E> \<pi>2 = Some \<sigma>\<^sub>2 \<longrightarrow>
-    \<pi>1 \<asymp> \<pi>2
-  )
-"
- apply (drule star_implies_star_left)
- apply (erule star_left.induct; auto)
-  apply (simp add: Ordered)
- apply (rename_tac \<E> \<E>' \<pi>1 \<sigma>\<^sub>1 \<pi>2 \<sigma>\<^sub>2)
- apply (blast dest: inclusive_preserved)
-done
-
-
-
-lemma runtime_paths_are_inclusive: "
-  \<lbrakk>
-    [[] \<mapsto> \<langle>e;Map.empty;[]\<rangle>] \<rightarrow>* \<E>';
-    \<E>' \<pi>1' = Some \<sigma>\<^sub>1';
-    \<E>' \<pi>2' = Some \<sigma>\<^sub>2'
-  \<rbrakk> \<Longrightarrow> 
-  \<pi>1' \<asymp> \<pi>2'
-"
-by (blast dest: runtime_paths_are_inclusive')
-
-
-
-
-lemma runtime_send_paths_are_inclusive: "
-  \<lbrakk>
-    [[] \<mapsto> \<langle>e;Map.empty;[]\<rangle>] \<rightarrow>* \<E>';
-    is_send_path \<E>' c \<pi>1';
-    is_send_path \<E>' c \<pi>2'
-  \<rbrakk> \<Longrightarrow> 
-  \<pi>1' \<asymp> \<pi>2'
-"
-apply (unfold is_send_path.simps; auto)
-using runtime_paths_are_inclusive by blast
-
-
-*)
 
 inductive 
   dynamic_built_on_chan_var :: "(var \<rightharpoonup> val) \<Rightarrow> chan \<Rightarrow> var \<Rightarrow> bool" and
@@ -834,8 +589,29 @@ lemma call_return_balanced: "
 "
 using balanced.CallReturn balanced.Empty by fastforce
 
+inductive paths_congruent :: "control_path \<Rightarrow> abstract_path \<Rightarrow> bool" where
+  Empty: "
+    paths_congruent [] []
+  " |
+  Next: "
+    paths_congruent \<pi> path \<Longrightarrow>
+    paths_congruent (\<pi> ;; (LNext x)) (path @ [(NLet x, ENext)])
+  " |
+  Spawn: "
+    paths_congruent \<pi> path \<Longrightarrow>
+    paths_congruent (\<pi> ;; (LSpawn x)) (path @ [(NLet x, ESpawn)])
+  " |
+  Call: "
+    paths_congruent \<pi> path \<Longrightarrow>
+    paths_congruent (\<pi> ;; (LCall x)) (path @ [(NLet x, ECall)])
+  "  |
+  Return: "
+    paths_congruent \<pi> (path @ (NLet x, ECall) # path') \<Longrightarrow>
+    abstract_balanced path' \<Longrightarrow>
+    paths_congruent (\<pi> ;; (LReturn y)) (path @ (NLet x, ECall) # path' @ [(NResult y, EReturn x)])
+  " 
 
-inductive paths_congruent_mod_chan :: "trace_pool * com_set \<Rightarrow> chan \<Rightarrow> control_path \<Rightarrow> static_path \<Rightarrow> bool" where
+inductive paths_congruent_mod_chan :: "trace_pool * com_set \<Rightarrow> chan \<Rightarrow> control_path \<Rightarrow> abstract_path \<Rightarrow> bool" where
   Unordered: "
     paths_congruent \<pi> pathx \<Longrightarrow>
     \<not> (prefix pathx path) \<Longrightarrow>
@@ -865,325 +641,6 @@ lemma no_empty_paths_congruent_mod_chan: "
   apply (erule paths_congruent.cases; auto)
 done
 
-(*
-lemma static_paths_of_same_run_inclusive_base: "
-  E0 = [[] \<mapsto> \<langle>e;Map.empty;[]\<rangle>] \<Longrightarrow>
-  E0 \<pi>1 \<noteq> None \<Longrightarrow>
-  E0 \<pi>2 \<noteq> None \<Longrightarrow>
-  paths_congruent_mod_chan (E0, {}) (Ch \<pi> xC) \<pi>1 path1 \<Longrightarrow> 
-  paths_congruent_mod_chan (E0, {}) (Ch \<pi> xC) \<pi>2 path2 \<Longrightarrow>
-  path1 \<asymp> path2
-"
-proof -
-  assume 
-    H1: "E0 = [[] \<mapsto> \<langle>e;Map.empty;[]\<rangle>]" and
-    H2: "E0 \<pi>1 \<noteq> None" and
-    H3: "E0 \<pi>2 \<noteq> None" and
-    H4: "paths_congruent_mod_chan (E0, {}) (Ch \<pi> xC) \<pi>1 path1" and
-    H5: "paths_congruent_mod_chan (E0, {}) (Ch \<pi> xC) \<pi>2 path2"
-  from H1 H2 H4 show 
-    "path1 \<asymp> path2" 
-    by (metis fun_upd_apply no_empty_paths_congruent_mod_chan)
-qed
-
-
-lemma paths_equal_implies_paths_inclusive: "
-  path1 = path2 \<Longrightarrow> path1 \<asymp> path2 
-"
-by (simp add: Prefix2)
-
-lemma paths_cong_preserved_under_reduction: "
-  paths_congruent (\<pi> ;; l) (path @ [n]) \<Longrightarrow>
-  paths_congruent \<pi> path"
-using paths_congruent.cases by fastforce
-
-
-lemma equal_concrete_paths_implies_unordered_or_equal_abstract_paths: "
-paths_congruent_mod_chan EH c \<pi> path1 \<Longrightarrow>
-paths_congruent_mod_chan EH c \<pi> path2 \<Longrightarrow>
-path1 = path2 \<or> (\<not> prefix path1 path2 \<and> \<not> prefix path2 path1)
-"
-sorry
-
-lemma path_cong_mod_chan_preserved_under_reduction: "
-paths_congruent_mod_chan (E', H') (Ch \<pi>C xC) (\<pi> ;; l) (path @ [n]) \<Longrightarrow>
-(E, H) \<rightarrow> (E', H') \<Longrightarrow>
-paths_congruent_mod_chan (E, H) (Ch \<pi>C xC) \<pi> path
-"
-sorry
-
-lemma leaf_prefix_exists: "
-  leaf E' (\<pi> ;; l) \<Longrightarrow>
-  (E, H) \<rightarrow> (E', H') \<Longrightarrow>
-  E \<pi> \<noteq> None
-"
-sorry
-
-
-lemma path_state_preserved_for_non_leaf: "
-(E, H) \<rightarrow> (E', H') \<Longrightarrow>
-E' (\<pi> ;; l) = Some \<sigma> \<Longrightarrow>
-\<not> leaf E \<pi> \<Longrightarrow>
-E (\<pi> ;; l) = Some \<sigma>
-"
-apply (erule concur_step.cases; auto; (erule seq_step.cases; auto)?)
-  apply presburger+
-  apply (metis append1_eq_conv fun_upd_other)
-  apply (metis butlast_snoc fun_upd_apply)
-done
-
-
-lemma static_paths_of_same_run_inclusive_step: "
-\<forall>\<pi>1 \<pi>2 path1 path2.
-  E \<pi>1 \<noteq> None \<longrightarrow>
-  E \<pi>2 \<noteq> None \<longrightarrow>
-  paths_congruent_mod_chan (E, H) (Ch \<pi>C xC) \<pi>1 path1 \<longrightarrow> 
-  paths_congruent_mod_chan (E, H) (Ch \<pi>C xC) \<pi>2 path2 \<longrightarrow> 
-  path1 \<asymp> path2 \<Longrightarrow>
-star_left op \<rightarrow> ([[] \<mapsto> \<langle>e;Map.empty;[]\<rangle>], {}) (E, H) \<Longrightarrow>
-(E, H) \<rightarrow> (E', H') \<Longrightarrow>
-E' \<pi>1 \<noteq> None \<Longrightarrow>
-E' \<pi>2 \<noteq> None \<Longrightarrow>
-paths_congruent_mod_chan (E', H') (Ch \<pi>C xC) \<pi>1 path1 \<Longrightarrow> 
-paths_congruent_mod_chan (E', H') (Ch \<pi>C xC) \<pi>2 path2 \<Longrightarrow>
-path1 \<asymp> path2 
-"
-(* TO DO: switch to ISAR style;
-
-   derive equal and unordered paths; 
-   derive inclusive paths
-
-*)
-
-proof ((case_tac "path1 = []"; (simp add: Prefix1)), (case_tac "path2 = []", (simp add: Prefix2)))
-  assume 
-    H1: "
-      \<forall>\<pi>1. (\<exists>y. E \<pi>1 = Some y) \<longrightarrow>
-      (\<forall>\<pi>2. (\<exists>y. E \<pi>2 = Some y) \<longrightarrow>
-      (\<forall>path1. paths_congruent_mod_chan (E, H) (Ch \<pi>C xC) \<pi>1 path1 \<longrightarrow>
-      (\<forall>path2. paths_congruent_mod_chan (E, H) (Ch \<pi>C xC) \<pi>2 path2 \<longrightarrow> 
-        path1 \<asymp> path2)))" and
-    H2: "star_left op \<rightarrow> ([[] \<mapsto> \<langle>e;Map.empty;[]\<rangle>], {}) (E, H)" and
-    H3: "(E, H) \<rightarrow> (E', H')" and
-    H4: "\<exists>y. E' \<pi>1 = Some y" and
-    H5: "\<exists>y. E' \<pi>2 = Some y " and
-    H6: "paths_congruent_mod_chan (E', H') (Ch \<pi>C xC) \<pi>1 path1" and
-    H7: "paths_congruent_mod_chan (E', H') (Ch \<pi>C xC) \<pi>2 path2" and
-    H8: "path1 \<noteq> []" and 
-    H9: "path2 \<noteq> []"
-
-  obtain \<sigma>1 where 
-    H10: "E' \<pi>1 = Some \<sigma>1"
-    using H4 by blast
-
-  obtain \<sigma>2 where 
-    H11: "E' \<pi>2 = Some \<sigma>2"
-    using H5 by blast
-
-  obtain \<pi>1x l1 path1x n1 where
-    H12: "\<pi>1x ;; l1 = \<pi>1" and
-    H13: "path1x @ [n1] = path1" and
-    H14: "paths_congruent_mod_chan (E, H) (Ch \<pi>C xC) \<pi>1x path1x" 
-  by (metis H3 H6 H8 append_butlast_last_id path_cong_mod_chan_preserved_under_reduction no_empty_paths_congruent_mod_chan)
-
-  obtain \<pi>2x l2 path2x n2 where
-    H15: "\<pi>2x ;; l2 = \<pi>2" and
-    H16: "path2x @ [n2] = path2" and
-    H17: "paths_congruent_mod_chan (E, H) (Ch \<pi>C xC) \<pi>2x path2x"
-  by (metis H3 H7 H9 append_butlast_last_id path_cong_mod_chan_preserved_under_reduction no_empty_paths_congruent_mod_chan)
-
-
-  have H18: "paths_congruent_mod_chan (E, H) (Ch \<pi>C xC) \<pi>1 path1" sorry
-
-  have H19: "paths_congruent_mod_chan (E, H) (Ch \<pi>C xC) \<pi>2 path2" sorry
-
-  show "path1 \<asymp> path2"
-  proof cases
-    assume L1H1: "leaf E \<pi>1x"
-    obtain \<sigma>1x where
-      L1H2: "E \<pi>1x = Some \<sigma>1x" using L1H1 leaf.simps by auto
-    show "path1 \<asymp> path2"
-    proof cases
-      assume L2H1: "leaf E \<pi>2x"
-      obtain \<sigma>2x where
-        L2H2: "E \<pi>2x = Some \<sigma>2x" using L2H1 leaf.simps by auto
-      have "path1x \<asymp> path2x"
-        using H1 H14 H17 L1H2 L2H2 by blast
-      (* inclusive definition fails in case of non-unique variable bindings *)
-      show "path1 \<asymp> path2" sorry
-    next
-      assume L2H1: "\<not> leaf E \<pi>2x"
-      have L2H2: "E \<pi>2 = Some \<sigma>2"
-        using H11 H15 H3 L2H1 path_state_preserved_for_non_leaf by blast
-      have L2H3: "path1x \<asymp> path2"
-        using H1 H14 H19 L1H2 L2H2 by auto
-
-      have L2H4: "\<not> strict_prefix \<pi>1x \<pi>2"
-        by (metis L1H1 L2H2 leaf.cases option.distinct(1))
-      show "path1 \<asymp> path2"
-      proof cases
-        assume L3H1: "prefix path1x path2"
-       (* inclusive definition fails in case of non-unique variable bindings *)
-        show "path1 \<asymp> path2" sorry
-      next
-        assume L3H1: "\<not> prefix path1x path2"
-        show "path1 \<asymp> path2"
-          by (metis H13 L2H3 L3H1 Prefix2 may_be_inclusive_preserved_under_unordered_extension prefix_prefix)
-      qed
-    qed
-
-  next
-    assume L1H1: "\<not> leaf E \<pi>1x"
-      have L1H2: "E \<pi>1 = Some \<sigma>1"
-        using H10 H12 H3 L1H1 path_state_preserved_for_non_leaf by blast
-    show "path1 \<asymp> path2"
-
-    proof cases
-      assume L2H1: "leaf E \<pi>2x"
-      obtain \<sigma>2x where
-        L2H2: "E \<pi>2x = Some \<sigma>2x" using L2H1 leaf.simps by auto
-      have L2H3: "path1 \<asymp> path2x"
-        using H1 H17 H18 L1H2 L2H2 by auto
-      show "path1 \<asymp> path2"
-      proof cases
-        assume L3H1: "prefix path2x path1"
-        show "path1 \<asymp> path2" sorry
-      next
-        assume L3H1: "\<not> prefix path2x path1"
-        show "path1 \<asymp> path2"
-          by (metis H16 L2H3 L3H1 Prefix1 may_be_inclusive_commut may_be_inclusive_preserved_under_unordered_extension prefix_prefix)
-      qed
-    next
-      assume L2H1: "\<not> leaf E \<pi>2x"
-      have L2H2: "E \<pi>2 = Some \<sigma>2"
-        using H11 H15 H3 L2H1 path_state_preserved_for_non_leaf by blast
-      show "path1 \<asymp> path2"
-        using H1 H18 H19 L1H2 L2H2 by blast
-    qed
-
-  qed
-
-qed
-(*
-apply ((case_tac "path1 = []"; (auto simp: Prefix1)), (case_tac "path2 = []", (auto simp: Prefix2)))
-apply (case_tac "path2 = []", (auto simp: Prefix2))
-apply (erule concur_step.cases; auto; (erule seq_step.cases; auto)?)
-  apply (case_tac "\<pi>1 = \<pi> ;; LReturn x\<^sub>\<kappa>"; auto; (case_tac "\<pi>2 = \<pi> ;; LReturn x\<^sub>\<kappa>"; auto)?)
-  apply (drule_tac x = \<pi> in spec; auto)
-  apply (drule_tac x = \<pi> in spec; auto)
-  apply (drule_tac x = "(butlast path1)" in spec; auto)
-  apply (metis append_butlast_last_id path_cong_mod_chan_preserved_under_reduction)
-  apply (drule_tac x = "(butlast path2)" in spec; auto)
-  apply (metis append_butlast_last_id path_cong_mod_chan_preserved_under_reduction)
-  apply (erule paths_congruent_mod_chan.cases; auto; (erule paths_congruent_mod_chan.cases; auto))
-  apply (erule paths_congruent.cases; auto; (erule paths_congruent.cases; auto); (erule nodes_congruent.cases))
-done
-*)
-
-lemma static_paths_of_same_run_inclusive: "
-  ([[] \<mapsto> \<langle>e;Map.empty;[]\<rangle>], {}) \<rightarrow>* (\<E>', H') \<Longrightarrow> 
-  \<E>' \<pi>1 \<noteq> None \<Longrightarrow> 
-  \<E>' \<pi>2 \<noteq> None \<Longrightarrow> 
-  paths_congruent_mod_chan (\<E>', H') (Ch \<pi> xC) \<pi>1 path1 \<Longrightarrow>
-  paths_congruent_mod_chan (\<E>', H') (Ch \<pi> xC) \<pi>2 path2 \<Longrightarrow>
-  path1 \<asymp> path2
-"
-proof -
-  assume
-    H1: "([[] \<mapsto> \<langle>e;Map.empty;[]\<rangle>], {}) \<rightarrow>* (\<E>', H')" and
-    H2: "\<E>' \<pi>1 \<noteq> None" and
-    H3: "\<E>' \<pi>2 \<noteq> None" and
-    H4: "paths_congruent_mod_chan (\<E>', H') (Ch \<pi> xC) \<pi>1 path1" and
-    H5: "paths_congruent_mod_chan (\<E>', H') (Ch \<pi> xC) \<pi>2 path2"
-
-  from H1 have
-    "star_left (op \<rightarrow>) ([[] \<mapsto> \<langle>e;Map.empty;[]\<rangle>], {}) (\<E>', H')" by (simp add: star_implies_star_left)
-  
-  then obtain X0 X' where 
-    H6: "X0 = ([[] \<mapsto> \<langle>e;Map.empty;[]\<rangle>], {})" 
-        "X' = (\<E>', H')" and
-    H7: "star_left (op \<rightarrow>) X0 X'" by auto
-
-  from H7 have 
-    H8: "
-      \<forall> \<E>' H' \<pi>1 \<pi>2 path1 path2.
-      X0 = ([[] \<mapsto> \<langle>e;Map.empty;[]\<rangle>], {}) \<longrightarrow> X' = (\<E>', H') \<longrightarrow>
-      \<E>' \<pi>1 \<noteq> None \<longrightarrow>
-      \<E>' \<pi>2 \<noteq> None \<longrightarrow>
-      paths_congruent_mod_chan (\<E>', H') (Ch \<pi> xC) \<pi>1 path1 \<longrightarrow>
-      paths_congruent_mod_chan (\<E>', H') (Ch \<pi> xC) \<pi>2 path2 \<longrightarrow>
-      path1 \<asymp> path2
-    "
-  proof induction
-    case (refl z)
-    then show ?case
-      using static_paths_of_same_run_inclusive_base by blast
-  next
-    case (step x y z)
-
-    {
-      fix \<E>' H' \<pi>1 \<pi>2 path1 path2
-      assume 
-        L2H1: "x = ([[] \<mapsto> \<langle>e;Map.empty;[]\<rangle>], {})" and
-        L2H2: "z = (\<E>', H')" and
-        L2H3: "\<E>' \<pi>1 \<noteq> None" and
-        L2H4: "\<E>' \<pi>2 \<noteq> None" and
-        L2H5: "paths_congruent_mod_chan (\<E>', H') (Ch \<pi> xC) \<pi>1 path1" and
-        L2H6: "paths_congruent_mod_chan (\<E>', H') (Ch \<pi> xC) \<pi>2 path2"
-
-      obtain \<E> H where 
-        L2H7: "y = (\<E>, H)" by (meson surj_pair)
-
-      from L2H1 L2H7 step.IH have 
-        L2H8: "
-          \<forall> \<pi>1 \<pi>2 path1 path2 . 
-          \<E> \<pi>1 \<noteq> None \<longrightarrow>
-          \<E> \<pi>2 \<noteq> None \<longrightarrow>
-          paths_congruent_mod_chan (\<E>, H) (Ch \<pi> xC) \<pi>1 path1 \<longrightarrow> 
-          paths_congruent_mod_chan (\<E>, H) (Ch \<pi> xC) \<pi>2 path2 \<longrightarrow> 
-          path1 \<asymp> path2 "
-        by blast
-
-      have 
-        "path1 \<asymp> path2"
-        using L2H1 L2H2 L2H3 L2H4 L2H5 L2H6 L2H7 L2H8 static_paths_of_same_run_inclusive_step step.hyps(1) step.hyps(2) by blast
-    }
-    then show ?case by blast
-  qed
-
-  from H2 H3 H4 H5 H6(1) H6(2) H8 show 
-    "path1 \<asymp> path2" by blast
-qed
-
-lemma is_send_path_implies_nonempty_pool: "
-  is_send_path \<E> (Ch \<pi>C xC) \<pi> \<Longrightarrow> 
-  \<E> \<pi> \<noteq> None
-"
-proof -
-  assume H1: "is_send_path \<E> (Ch \<pi>C xC) \<pi>"
-  
-  then have
-    H2: "
-      \<exists> x\<^sub>y x\<^sub>e e\<^sub>n \<rho> \<kappa>. \<E> \<pi> = Some (\<langle>LET x\<^sub>y = SYNC x\<^sub>e in e\<^sub>n;\<rho>;\<kappa>\<rangle>) 
-    " using is_send_path.simps by auto
-
-  then show 
-    "\<E> \<pi> \<noteq> None" by blast
-qed
-
-lemma send_static_paths_of_same_run_inclusive: "
-  ([[] \<mapsto> \<langle>e;Map.empty;[]\<rangle>], {}) \<rightarrow>* (\<E>', H') \<Longrightarrow> 
-  is_send_path \<E>' (Ch \<pi> xC) \<pi>1 \<Longrightarrow> 
-  is_send_path \<E>' (Ch \<pi> xC) \<pi>2 \<Longrightarrow> 
-  paths_congruent_mod_chan (\<E>', H') (Ch \<pi> xC) \<pi>1 path1 \<Longrightarrow>
-  paths_congruent_mod_chan (\<E>', H') (Ch \<pi> xC) \<pi>2 path2 \<Longrightarrow>
-  path1 \<asymp> path2
-"
-using is_send_path_implies_nonempty_pool static_paths_of_same_run_inclusive by fastforce
-*)
-
-
-
 
 lemma send_path_equality_sound: "
   path1 = path2 \<Longrightarrow>
@@ -1196,7 +653,7 @@ lemma send_path_equality_sound: "
 "
 sorry
 (*
-lemma send_static_paths_equal_unordered_implies_dynamic_paths_equal: "
+lemma send_abstract_paths_equal_unordered_implies_dynamic_paths_equal: "
 pathSync = pathSynca \<or> (\<not> pathSynca \<asymp> pathSync) \<Longrightarrow> 
 
 ([[] \<mapsto> \<langle>e;Map.empty;[]\<rangle>], {}) \<rightarrow>* (\<E>', H') \<Longrightarrow>
@@ -1208,7 +665,7 @@ paths_congruent_mod_chan (\<E>', H') (Ch \<pi> xC) \<pi>\<^sub>2 pathSynca \<Lon
 
 \<pi>\<^sub>1 = \<pi>\<^sub>2
 "
-by (simp add: send_path_equality_sound send_static_paths_of_same_run_unordered)
+by (simp add: send_path_equality_sound send_abstract_paths_of_same_run_unordered)
 *)
 (* END *)
 
@@ -1231,60 +688,6 @@ lemma isnt_path_sound: "
 sorry
 
 
-lemma isnt_send_evt_sound: "
-  \<lbrakk>
-    \<rho>\<^sub>y x\<^sub>e = Some (VClosure (Send_Evt x\<^sub>s\<^sub>c x\<^sub>m) \<rho>\<^sub>e);
-    ([[] \<mapsto> \<langle>e;Map.empty;[]\<rangle>], {}) \<rightarrow>* (\<E>', H');
-    \<E>' \<pi>\<^sub>y = Some (\<langle>LET x\<^sub>y = SYNC x\<^sub>e in e\<^sub>y;\<rho>\<^sub>y;\<kappa>\<^sub>y\<rangle>);
-    (V, C) \<Turnstile>\<^sub>e e
-  \<rbrakk> \<Longrightarrow>
-  {^Send_Evt x\<^sub>s\<^sub>c x\<^sub>m} \<subseteq> V x\<^sub>e
-"
-  apply (drule values_not_bound_sound; assumption?; auto)
-done
-
-lemma isnt_send_chan_sound: "
-  \<lbrakk>
-    \<rho>\<^sub>e x\<^sub>s\<^sub>c = Some (VChan (Ch \<pi> xC));
-    \<rho>\<^sub>y x\<^sub>e = Some (VClosure (Send_Evt x\<^sub>s\<^sub>c x\<^sub>m) \<rho>\<^sub>e);
-    \<E>' \<pi>\<^sub>y = Some (\<langle>LET x\<^sub>y = SYNC x\<^sub>e in e\<^sub>y;\<rho>\<^sub>y;\<kappa>\<^sub>y\<rangle>);
-    ([[] \<mapsto> \<langle>e;Map.empty;[]\<rangle>], {}) \<rightarrow>* (\<E>', H');
-    (V, C) \<Turnstile>\<^sub>e e
-  \<rbrakk> \<Longrightarrow> 
-  ^Chan xC \<in> V x\<^sub>s\<^sub>c
-"
- apply (frule may_be_static_eval_to_pool)
- apply (drule may_be_static_eval_preserved_under_concur_step_star[of _ _ _ ]; assumption?)
- apply (erule may_be_static_eval_pool.cases; auto)
- apply (drule spec[of _ \<pi>\<^sub>y], drule spec[of _ "\<langle>LET x\<^sub>y = SYNC x\<^sub>e in e\<^sub>y;\<rho>\<^sub>y;\<kappa>\<^sub>y\<rangle>"], simp)
- apply (erule may_be_static_eval_state.cases; auto)
- apply (erule may_be_static_eval_env.cases; auto)
- apply (drule spec[of _ x\<^sub>e], drule spec[of _ "(VClosure (Send_Evt x\<^sub>s\<^sub>c x\<^sub>m) \<rho>\<^sub>e)"]; simp)
- apply (erule conjE)
- apply (erule may_be_static_eval_value.cases; auto)
- apply (erule may_be_static_eval_env.cases; auto)
- apply (drule spec[of _ x\<^sub>s\<^sub>c], drule spec[of _ "(VChan (Ch \<pi> xC))"]; simp)
-done
-
-lemma isnt_send_site_sound: "
-  \<E>' \<pi>Sync = Some (\<langle>LET x\<^sub>y = SYNC x\<^sub>e in e\<^sub>n;\<rho>;\<kappa>\<rangle>) \<Longrightarrow>
-  \<rho> x\<^sub>e = Some (VClosure (Send_Evt x\<^sub>s\<^sub>c x\<^sub>m) \<rho>\<^sub>e) \<Longrightarrow>
-  \<rho>\<^sub>e x\<^sub>s\<^sub>c = Some (VChan (Ch \<pi>C xC)) \<Longrightarrow>
-  ([[] \<mapsto> \<langle>e;Map.empty;[]\<rangle>], {}) \<rightarrow>* (\<E>', H') \<Longrightarrow> 
-  (V, C) \<Turnstile>\<^sub>e e \<Longrightarrow>
-  may_be_static_send_node_label V e xC (NLet x\<^sub>y)
-"
- apply (unfold may_be_static_send_node_label.simps; auto)
- apply (rule exI[of _ x\<^sub>s\<^sub>c]; auto)
- apply (auto simp: isnt_send_chan_sound)
- apply (rule exI[of _ x\<^sub>m]; auto?)
- apply (rule exI[of _ x\<^sub>e]; auto?)
- apply (blast dest: isnt_send_evt_sound)
- apply (rule exI; auto?)
- apply (erule isnt_exp_sound; auto)
-done
-
-
 lemma isnt_send_path_sound: "
   is_send_path \<E>' (Ch \<pi>C xC) \<pi>Sync \<Longrightarrow>
   ([[] \<mapsto> \<langle>e;Map.empty;[]\<rangle>], {}) \<rightarrow>* (\<E>', H') \<Longrightarrow> 
@@ -1304,31 +707,18 @@ lemma isnt_send_path_sound: "
   )
 done
 
-(* END PATH SOUND *)
-
-
 
 theorem one_shot_sound': "
-  every_two_static_paths (may_be_static_live_path V F Ln Lx (NLet xC) (may_be_static_send_node_label V e xC)) singular \<Longrightarrow>
+  every_two (may_be_static_live_path V F Ln Lx (NLet xC) (may_be_static_send_node_label V e xC)) singular \<Longrightarrow>
   static_chan_liveness V Ln Lx xC e \<Longrightarrow>
   static_flow_set V F (may_be_static_recv_node_label V e) e \<Longrightarrow>
   (V, C) \<Turnstile>\<^sub>e e \<Longrightarrow>
   ([[] \<mapsto> \<langle>e;Map.empty;[]\<rangle>], {}) \<rightarrow>* (\<E>', H') \<Longrightarrow> 
   every_two_dynamic_paths (is_send_path \<E>' (Ch \<pi> xC)) op =
 "
-apply (simp add: every_two_dynamic_paths.simps every_two_static_paths.simps singular.simps; auto)
+apply (simp add: every_two_dynamic_paths.simps every_two.simps singular.simps; auto)
 apply (metis isnt_send_path_sound send_path_equality_sound)
 done
-(*
- apply (simp add: every_two_dynamic_paths.simps every_two_static_paths.simps singular.simps; auto)
- apply (frule_tac \<pi>Sync = \<pi>\<^sub>1 in isnt_send_path_sound; auto)
- apply (drule_tac x = pathSync in spec)
- apply (frule_tac \<pi>Sync = \<pi>\<^sub>2 in isnt_send_path_sound; auto?)
- apply (drule_tac x = pathSynca in spec)
- apply (erule impE, simp)
- apply (simp add: send_static_paths_equal_unordered_implies_dynamic_paths_equal)
- done
-*)
 
 
 
@@ -1345,23 +735,17 @@ theorem one_shot_sound: "
  apply (simp add: one_shot_sound')
 done
 
-(*
-TO DO LATER:
-*)
-
 theorem noncompetitive_send_to_ordered_send: "
-  every_two_static_paths (may_be_static_live_path V F Ln Lx (NLet xC) (may_be_static_send_node_label V e xC)) noncompetitive \<Longrightarrow>
+  every_two (may_be_static_live_path V F Ln Lx (NLet xC) (may_be_static_send_node_label V e xC)) noncompetitive \<Longrightarrow>
   static_chan_liveness V Ln Lx xC e \<Longrightarrow>
   static_flow_set V F (may_be_static_recv_node_label V e) e \<Longrightarrow>
   (V, C) \<Turnstile>\<^sub>e e \<Longrightarrow>
   ([[] \<mapsto> \<langle>e;Map.empty;[]\<rangle>], {}) \<rightarrow>* (\<E>', H') \<Longrightarrow>
   every_two_dynamic_paths (is_send_path \<E>' (Ch \<pi> xC)) ordered
 "
-sorry
-(*
+
 apply (simp add: every_two_dynamic_paths.simps noncompetitive.simps; auto)
-using isnt_send_path_sound runtime_send_paths_are_inclusive by blast
-*)
+sorry
 
 theorem fan_out_sound: "
   \<lbrakk>
@@ -1377,7 +761,7 @@ theorem fan_out_sound: "
 done
 
 lemma noncompetitive_recv_to_ordered_recv: "
-   every_two_static_paths (may_be_static_live_path V F Ln Lx (NLet xC) (may_be_static_recv_node_label V e xC)) noncompetitive \<Longrightarrow>
+   every_two (may_be_static_live_path V F Ln Lx (NLet xC) (may_be_static_recv_node_label V e xC)) noncompetitive \<Longrightarrow>
    static_flow_set V F (may_be_static_recv_node_label V e) e \<Longrightarrow>
    (V, C) \<Turnstile>\<^sub>e e \<Longrightarrow>
    ([[] \<mapsto> \<langle>e;Map.empty;[]\<rangle>], {}) \<rightarrow>* (\<E>', H') \<Longrightarrow>
@@ -1414,121 +798,4 @@ theorem one_to_one_sound: "
 done
 
 
-
-
-(*
-lemma paths_cong_mod_chan_preserved_under_reduction: "
-(suffix \<pi> (\<pi>C ;; (LNext xC)) \<and> suffix path [(NLet xC, ENext)] \<or>
-  True) \<Longrightarrow>
-paths_congruent_mod_chan EH' (Ch \<pi>C xC) (\<pi> ;; l) (path @ [n]) \<Longrightarrow>
-E \<pi> \<noteq> None \<Longrightarrow>
-paths_congruent_mod_chan (E, H) (Ch \<pi>C xC) \<pi> path"
-proof -
-  assume
-    H1: "E \<pi> \<noteq> None" and
-    H2: "\<pi> \<noteq> []" "path \<noteq> []" and
-    H3: "paths_congruent_mod_chan EH' c (\<pi> ;; l) (path @ [n])"
-
-  from H3
-  show "paths_congruent_mod_chan (E, H) c \<pi> path"
-  proof cases
-
-    case (Chan xC \<pi>X E' \<pi>C H')
-
-    have 
-      H4: "\<pi> ;; l = \<pi>C @ (butlast (LNext xC # \<pi>X)) ;; l"
-      by (metis butlast_append butlast_snoc list.simps(3) local.Chan(3))
-    
-    have 
-      H5: "paths_congruent ((butlast (LNext xC # \<pi>X)) ;; l) (path @ [n])"
-      by (metis append_butlast_last_id last_ConsL last_appendR list.simps(3) local.Chan(3) local.Chan(4))
-
-    have 
-      H6: "butlast (LNext xC # \<pi>X) \<noteq> []"
-      by (metis H2(2) H5 paths_congruent.cases snoc_eq_iff_butlast)
-
-    have 
-      H7: "paths_congruent (butlast (LNext xC # \<pi>X)) path"
-      using H2(2) H5 H6 paths_cong_preserved_under_reduction by blast
-
-    have 
-      H8: "paths_congruent (LNext xC # (butlast \<pi>X)) path"
-      by (metis H6 H7 butlast.simps(2))
-
-    have L2H10: "\<pi> = \<pi>C @ butlast (LNext xC # \<pi>X)"
-    using H4 by blast
-
-    have "paths_congruent_mod_chan (E, H) (Ch \<pi>C xC) \<pi> path"
-    using H1 H6 H8 L2H10 paths_congruent_mod_chan.Chan by auto
-     
-    then show "paths_congruent_mod_chan (E, H) c \<pi> path"
-    by (simp add: local.Chan(2))
-
-  next
-    case (Sync \<pi>Suffix pathSuffix E' \<pi>R xR \<rho>RY \<pi>S xS xSE eSY \<rho>SY \<kappa>SY xRE eRY \<kappa>RY H' pathPre)
-
-    
-    then show "paths_congruent_mod_chan (E, H) c \<pi> path"
-    proof cases
-      assume L1H1: "pathSuffix = []"
-
-      have L1H2: "path = pathPre @ [(NLet xS, ESend xSE)]"
-        using L1H1 local.Sync(3) by auto
-
-      have L1H3: "\<pi>Suffix = []"
-        using L1H1 local.Sync(4) paths_congruent.cases by blast
-
-      have L1H3: "\<pi> = \<pi>R"
-        using L1H3 local.Sync(2) by blast
-
-      have "paths_congruent_mod_chan (E, H) c \<pi>R (pathPre @ [(NLet xS, ESend xSE)])" sorry
-
-      then show ?thesis sorry
-    next
-      assume L1H1: "pathSuffix \<noteq> []"
-
-      have 
-        L1H2: "path = pathPre @ (NLet xS, ESend xSE) # (NLet xR, ENext) # (butlast pathSuffix)"
-        by (metis L1H1 butlast.simps(2) butlast_append butlast_snoc list.simps(3) local.Sync(3))
-      
-      have L1H3: "\<pi>Suffix \<noteq> []"
-        using local.Sync(4) paths_congruent.cases sorry
-
-      have L1H4: "\<pi> = \<pi>R @ LNext xR # (butlast \<pi>Suffix)"
-        by (metis L1H3 butlast.simps(2) butlast_append butlast_snoc list.distinct(1) local.Sync(2))
-
-      show ?thesis
-      proof cases
-        assume 
-          L2H1: "(butlast pathSuffix) = []"
-
-        have 
-          L2H2: "path = pathPre @ [(NLet xS, ESend xSE), (NLet xR, ENext)]"
-          by (simp add: L1H2 L2H1)
-
-        have 
-          L2H3: "(butlast \<pi>Suffix) = []" sorry
-
-        have L2H4: "\<pi> = \<pi>R @ [LNext xR]" by (simp add: L1H4 L2H3)
-
-        have 
-          "paths_congruent_mod_chan (E, H) c (\<pi>R @ [LNext xR]) (pathPre @ [(NLet xS, ESend xSE), (NLet xR, ENext)])" sorry
-
-        then show ?thesis
-          by (simp add: L2H2 L2H4)
-      next
-        assume "(butlast pathSuffix) \<noteq> []"
-        then show ?thesis sorry
-      qed
-    qed
-  (*next
-    third case
-  *)
-  qed
-qed
-*)
-
-
 end
-
-*)
