theory/Static_Communication_Analysis.thy
@@ -1,0 +1,181 @@
+theory Static_Communication_Analysis
+  imports Main Syntax 
+    Dynamic_Semantics Static_Semantics
+    Dynamic_Communication_Analysis
+begin
+
+inductive every_two :: "('a \<Rightarrow> bool) \<Rightarrow> ('a \<Rightarrow> 'a \<Rightarrow> bool) \<Rightarrow> bool" where
+  pred: "
+    (\<forall> path1 path2 . P path1 \<longrightarrow> P path2 \<longrightarrow> 
+      R path1 path2) \<Longrightarrow>
+    every_two P R
+  "
+
+datatype node_label = NLet var | NResult var
+
+fun nodeLabel :: "exp \<Rightarrow> node_label" where
+  "nodeLabel (LET x = b in e) = NLet x" |
+  "nodeLabel (RESULT y) = NResult y"
+
+type_synonym node_set = "node_label set"
+
+type_synonym node_map = "node_label \<Rightarrow> var set"
+
+inductive may_be_static_send_node_label :: "abstract_value_env \<Rightarrow> exp \<Rightarrow> var \<Rightarrow> node_label \<Rightarrow> bool" where
+  Sync: "
+    {^Chan xC} \<subseteq> V xSC \<Longrightarrow>
+    {^Send_Evt xSC xM} \<subseteq> V xE \<Longrightarrow>
+    is_super_exp e (LET x = SYNC xE in e') \<Longrightarrow>
+    may_be_static_send_node_label V e xC (NLet x)
+  "
+
+inductive may_be_static_recv_node_label :: "abstract_value_env \<Rightarrow> exp \<Rightarrow> var \<Rightarrow> node_label \<Rightarrow> bool" where
+  Sync: "
+    {^Chan xC} \<subseteq> V xRC \<Longrightarrow>
+    {^Recv_Evt xRC} \<subseteq> V xE \<Longrightarrow>
+    is_super_exp e (LET x = SYNC xE in e') \<Longrightarrow>
+    may_be_static_recv_node_label V e xC (NLet x)
+  "
+
+
+
+lemma path_state_preserved_for_non_leaf: "
+(E, H) \<rightarrow> (E', H') \<Longrightarrow>
+E' (\<pi> ;; l) = Some \<sigma> \<Longrightarrow>
+\<not> leaf E \<pi> \<Longrightarrow>
+E (\<pi> ;; l) = Some \<sigma>
+"
+apply (erule concur_step.cases; auto; (erule seq_step.cases; auto)?)
+  apply presburger+
+  apply (metis append1_eq_conv fun_upd_other)
+  apply (metis butlast_snoc fun_upd_apply)
+done
+
+
+lemma spawn_point: "
+  (E, H) \<rightarrow> (E', H') \<Longrightarrow>
+  leaf E \<pi> \<Longrightarrow>
+  E' (\<pi> ;; l1) = Some \<sigma>1 \<Longrightarrow>
+  E' (\<pi> ;; l2) = Some \<sigma>2 \<Longrightarrow>
+  l1 = l2 \<or> 
+  (\<exists> x . l1 = (LNext x) \<and> l2 = (LSpawn x)) \<or>
+  (\<exists> x . l1 = (LSpawn x) \<and> l2 = (LNext x))
+"
+apply (erule concur_step.cases; auto; (erule seq_step.cases; auto)?)
+  apply (metis leaf.cases option.distinct(1) strict_prefixI')
+  apply (metis leaf.cases option.distinct(1) strict_prefixI')
+  apply (metis leaf.cases option.distinct(1) strict_prefixI')
+  apply (metis leaf.cases option.distinct(1) strict_prefixI')
+  apply (metis leaf.cases option.distinct(1) strict_prefixI')
+  apply (metis leaf.cases option.distinct(1) strict_prefixI')
+  apply (metis leaf.cases option.distinct(1) strict_prefixI')
+  apply (metis (mono_tags, lifting) append1_eq_conv fun_upd_apply leaf.cases option.distinct(1) strict_prefixI')
+  apply (smt butlast_snoc exp.inject(1) fun_upd_apply last_snoc leaf.cases option.distinct(1) option.inject state.inject strict_prefixI')
+done
+
+lemma isnt_send_evt_sound: "
+  \<lbrakk>
+    \<rho>\<^sub>y x\<^sub>e = Some (VClosure (Send_Evt x\<^sub>s\<^sub>c x\<^sub>m) \<rho>\<^sub>e);
+    ([[] \<mapsto> \<langle>e;Map.empty;[]\<rangle>], {}) \<rightarrow>* (\<E>', H');
+    \<E>' \<pi>\<^sub>y = Some (\<langle>LET x\<^sub>y = SYNC x\<^sub>e in e\<^sub>y;\<rho>\<^sub>y;\<kappa>\<^sub>y\<rangle>);
+    (V, C) \<Turnstile>\<^sub>e e
+  \<rbrakk> \<Longrightarrow>
+  {^Send_Evt x\<^sub>s\<^sub>c x\<^sub>m} \<subseteq> V x\<^sub>e
+"
+  apply (drule values_not_bound_sound; assumption?; auto)
+done
+
+lemma isnt_recv_evt_sound: "
+  \<lbrakk>
+    \<rho>\<^sub>y x\<^sub>e = Some (VClosure (Recv_Evt x\<^sub>r\<^sub>c) \<rho>\<^sub>e);
+    ([[] \<mapsto> \<langle>e;Map.empty;[]\<rangle>], {}) \<rightarrow>* (\<E>', H');
+    \<E>' \<pi>\<^sub>y = Some (\<langle>LET x\<^sub>y = SYNC x\<^sub>e in e\<^sub>y;\<rho>\<^sub>y;\<kappa>\<^sub>y\<rangle>);
+    (V, C) \<Turnstile>\<^sub>e e
+  \<rbrakk> \<Longrightarrow>
+  {^Recv_Evt x\<^sub>r\<^sub>c} \<subseteq> V x\<^sub>e
+"
+  apply (drule values_not_bound_sound; assumption?; auto)
+done
+
+lemma isnt_send_chan_sound: "
+  \<lbrakk>
+    \<rho>\<^sub>e x\<^sub>s\<^sub>c = Some (VChan (Ch \<pi> xC));
+    \<rho>\<^sub>y x\<^sub>e = Some (VClosure (Send_Evt x\<^sub>s\<^sub>c x\<^sub>m) \<rho>\<^sub>e);
+    \<E>' \<pi>\<^sub>y = Some (\<langle>LET x\<^sub>y = SYNC x\<^sub>e in e\<^sub>y;\<rho>\<^sub>y;\<kappa>\<^sub>y\<rangle>);
+    ([[] \<mapsto> \<langle>e;Map.empty;[]\<rangle>], {}) \<rightarrow>* (\<E>', H');
+    (V, C) \<Turnstile>\<^sub>e e
+  \<rbrakk> \<Longrightarrow> 
+  ^Chan xC \<in> V x\<^sub>s\<^sub>c
+"
+ apply (frule may_be_static_eval_to_pool)
+ apply (drule may_be_static_eval_preserved_under_concur_step_star[of _ _ _ ]; assumption?)
+ apply (erule may_be_static_eval_pool.cases; auto)
+ apply (drule spec[of _ \<pi>\<^sub>y], drule spec[of _ "\<langle>LET x\<^sub>y = SYNC x\<^sub>e in e\<^sub>y;\<rho>\<^sub>y;\<kappa>\<^sub>y\<rangle>"], simp)
+ apply (erule may_be_static_eval_state.cases; auto)
+ apply (erule may_be_static_eval_env.cases; auto)
+ apply (drule spec[of _ x\<^sub>e], drule spec[of _ "(VClosure (Send_Evt x\<^sub>s\<^sub>c x\<^sub>m) \<rho>\<^sub>e)"]; simp)
+ apply (erule conjE)
+ apply (erule may_be_static_eval_value.cases; auto)
+ apply (erule may_be_static_eval_env.cases; auto)
+ apply (drule spec[of _ x\<^sub>s\<^sub>c], drule spec[of _ "(VChan (Ch \<pi> xC))"]; simp)
+done
+
+lemma isnt_recv_chan_sound: "
+  \<lbrakk>
+    \<rho>\<^sub>e x\<^sub>r\<^sub>c = Some (VChan (Ch \<pi> xC));
+    \<rho>\<^sub>y x\<^sub>e = Some (VClosure (Recv_Evt x\<^sub>r\<^sub>c) \<rho>\<^sub>e);
+    \<E>' \<pi>\<^sub>y = Some (\<langle>LET x\<^sub>y = SYNC x\<^sub>e in e\<^sub>y;\<rho>\<^sub>y;\<kappa>\<^sub>y\<rangle>);
+    ([[] \<mapsto> \<langle>e;Map.empty;[]\<rangle>], {}) \<rightarrow>* (\<E>', H');
+    (V, C) \<Turnstile>\<^sub>e e
+  \<rbrakk> \<Longrightarrow> 
+  ^Chan xC \<in> V x\<^sub>r\<^sub>c
+"
+ apply (frule may_be_static_eval_to_pool)
+ apply (drule may_be_static_eval_preserved_under_concur_step_star[of _ _ _ ]; assumption?)
+ apply (erule may_be_static_eval_pool.cases; auto)
+ apply (drule spec[of _ \<pi>\<^sub>y], drule spec[of _ "\<langle>LET x\<^sub>y = SYNC x\<^sub>e in e\<^sub>y;\<rho>\<^sub>y;\<kappa>\<^sub>y\<rangle>"], simp)
+ apply (erule may_be_static_eval_state.cases; auto)
+ apply (erule may_be_static_eval_env.cases; auto)
+ apply (drule spec[of _ x\<^sub>e], drule spec[of _ "(VClosure (Recv_Evt x\<^sub>r\<^sub>c) \<rho>\<^sub>e)"]; simp)
+ apply (erule conjE)
+ apply (erule may_be_static_eval_value.cases; auto)
+ apply (erule may_be_static_eval_env.cases; auto)
+ apply (drule spec[of _ x\<^sub>r\<^sub>c], drule spec[of _ "(VChan (Ch \<pi> xC))"]; simp)
+done
+
+lemma isnt_send_site_sound: "
+  \<E>' \<pi>Sync = Some (\<langle>LET x\<^sub>y = SYNC x\<^sub>e in e\<^sub>n;\<rho>;\<kappa>\<rangle>) \<Longrightarrow>
+  \<rho> x\<^sub>e = Some (VClosure (Send_Evt x\<^sub>s\<^sub>c x\<^sub>m) \<rho>\<^sub>e) \<Longrightarrow>
+  \<rho>\<^sub>e x\<^sub>s\<^sub>c = Some (VChan (Ch \<pi>C xC)) \<Longrightarrow>
+  ([[] \<mapsto> \<langle>e;Map.empty;[]\<rangle>], {}) \<rightarrow>* (\<E>', H') \<Longrightarrow> 
+  (V, C) \<Turnstile>\<^sub>e e \<Longrightarrow>
+  may_be_static_send_node_label V e xC (NLet x\<^sub>y)
+"
+ apply (unfold may_be_static_send_node_label.simps; auto)
+ apply (rule exI[of _ x\<^sub>s\<^sub>c]; auto)
+ apply (auto simp: isnt_send_chan_sound)
+ apply (rule exI[of _ x\<^sub>m]; auto?)
+ apply (rule exI[of _ x\<^sub>e]; auto?)
+ apply (blast dest: isnt_send_evt_sound)
+ apply (rule exI; auto?)
+ apply (erule isnt_exp_sound; auto)
+done
+
+lemma isnt_recv_site_sound: "
+  \<E>' \<pi>Sync = Some (\<langle>LET x\<^sub>y = SYNC x\<^sub>e in e\<^sub>n;\<rho>;\<kappa>\<rangle>) \<Longrightarrow>
+  \<rho> x\<^sub>e = Some (VClosure (Recv_Evt x\<^sub>r\<^sub>c) \<rho>\<^sub>e) \<Longrightarrow>
+  \<rho>\<^sub>e x\<^sub>r\<^sub>c = Some (VChan (Ch \<pi>C xC)) \<Longrightarrow>
+  ([[] \<mapsto> \<langle>e;Map.empty;[]\<rangle>], {}) \<rightarrow>* (\<E>', H') \<Longrightarrow> 
+  (V, C) \<Turnstile>\<^sub>e e \<Longrightarrow>
+  may_be_static_recv_node_label V e xC (NLet x\<^sub>y)
+"
+ apply (unfold may_be_static_recv_node_label.simps; auto)
+ apply (rule exI[of _ x\<^sub>r\<^sub>c]; auto)
+ apply (auto simp: isnt_recv_chan_sound)
+ apply (rule exI[of _ x\<^sub>e]; auto?)
+ apply (blast dest: isnt_recv_evt_sound)
+ apply (rule exI; auto?)
+ apply (erule isnt_exp_sound; auto)
+done
+
+end
